DynamoDbItemEncryptor/test/TestFixtures.dfy
@@ -10,8 +10,9 @@ module TestFixtures {
   import MaterialProviders
   import Types = AwsCryptographyDynamoDbItemEncryptorTypes
   import DynamoDbItemEncryptor
+  import CTypes = AwsCryptographyStructuredEncryptionTypes
 
-  const EXPECTED_STUBBED_BLOB : seq<uint8> := [0x21, 0x64, 0x6c, 0x72, 0x6f, 0x77, 0x20, 0x2c, 0x6f, 0x6c, 0x6c, 0x65, 0x68];
+  //const EXPECTED_STUBBED_BLOB : seq<uint8> := [0x21, 0x64, 0x6c, 0x72, 0x6f, 0x77, 0x20, 0x2c, 0x6f, 0x6c, 0x6c, 0x65, 0x68];
 
   method GetStaticKeyring()
       returns (keyring: AwsCryptographyMaterialProvidersTypes.IKeyring)
@@ -30,23 +31,52 @@ module TestFixtures {
     );
   }
 
-  method GetDynamoDbItemEncryptor()
-      returns (encryptor: DynamoDbItemEncryptor.DynamoDbItemEncryptorClient)
+  function method GetAttributeActions() : Types.AttributeActions {
+    map["bar" := CTypes.SIGN_ONLY, "encrypt" := CTypes.ENCRYPT_AND_SIGN, "sign" := CTypes.SIGN_ONLY, "nothing" := CTypes.DO_NOTHING]
+  }
+
+
+  method GetEncryptorConfig() returns (output : Types.DynamoDbItemEncryptorConfig) {
+    var keyring := GetStaticKeyring();
+    output := Types.DynamoDbItemEncryptorConfig(
+      tableName := "foo",
+      partitionKeyName := "bar",
+      sortKeyName := None(),
+      attributeActions := GetAttributeActions(),
+      allowedUnauthenticatedAttributes := None(),
+      allowedUnauthenticatedAttributePrefix := None(),
+      keyring := Some(keyring),
+      cmm := None()
+    );
+  }
+
+  method GetDynamoDbItemEncryptorFrom(config : Types.DynamoDbItemEncryptorConfig)
+    returns (encryptor: DynamoDbItemEncryptor.DynamoDbItemEncryptorClient)
     ensures encryptor.ValidState()
     ensures fresh(encryptor)
     ensures fresh(encryptor.Modifies)
   {
     var keyring := GetStaticKeyring();
     var encryptorConfig := Types.DynamoDbItemEncryptorConfig(
-      tableName := "foo",
-      partitionKeyName := "bar",
-      sortKeyName := None(),
-      attributeActions := map[],
-      allowedUnauthenticatedAttributes := None(),
-      allowedUnauthenticatedAttributePrefix := None(),
+      tableName := config.tableName,
+      partitionKeyName := config.partitionKeyName,
+      sortKeyName := config.sortKeyName,
+      attributeActions := config.attributeActions,
+      allowedUnauthenticatedAttributes := config.allowedUnauthenticatedAttributes,
+      allowedUnauthenticatedAttributePrefix := config.allowedUnauthenticatedAttributePrefix,
       keyring := Some(keyring),
       cmm := None()
     );
     encryptor :- expect DynamoDbItemEncryptor.DynamoDbItemEncryptor(encryptorConfig);
+  }
+
+  method GetDynamoDbItemEncryptor()
+      returns (encryptor: DynamoDbItemEncryptor.DynamoDbItemEncryptorClient)
+    ensures encryptor.ValidState()
+    ensures fresh(encryptor)
+    ensures fresh(encryptor.Modifies)
+  {
+    var config := GetEncryptorConfig();
+    encryptor := GetDynamoDbItemEncryptorFrom(config);
   }
 }
